theories/Imp2Clight.v
@@ -7,7 +7,7 @@ Require Import Any.
 Require Import ModSem.
 Require Import Imp.
 
-From compcert Require Import AST Integers Ctypes Clight Globalenvs.
+From compcert Require Import AST Integers Ctypes Clight Globalenvs Linking.
 
 Import Int.
 
@@ -27,6 +27,8 @@ Section Compile.
   (*   forall (intval : Z), *)
   (*     ((Zneg xH) < intval < modulus)%Z. *)
 
+  (* compile each module indiv, 
+     prove behavior refinement for whole (closed) prog after linking *)
   Context `{Σ: GRA.t}.
   Variable src : Mod.t.
   Variable src_ge : SkEnv.t.
@@ -36,13 +38,28 @@ Section Compile.
   Context {s2p : string -> ident}.
   Context {to_long : Z -> int64}.
 
+  (* initial gdefs = Imp.module, 
+     contains single module's glob vars & internal funs. *)
+  (* compile_stmt updates gdefs to include syscall defs. *)
+  (* external funs (not syscall) : in other mod (resolved by linking) / 
+     syscall : update gdefs dynamically by syntax *)
+  (* no external variables: with weak typing, can resort to linking *)
+  (* alloc/free should remain external (EF_malloc, EF_free)
+     -> memory mod is not compiled with other Imps, 
+     load/store are compiled in other way, so OK.
+     cmp: ?? *)
+  Let tgt_gdefs := list (ident * globdef (Ctypes.fundef function) type).
+
   Let Tlong0 :=
     (Tlong Signed noattr).
 
   Let Tptr0 tgt :=
     (Tpointer tgt noattr).
 
-  Let string_key {T} l x : option T :=
+  Definition ident_key {T} id l : option T :=
+    SetoidList.findA (Pos.eqb id) l.
+
+  Definition string_key {T} l x : option T :=
     SetoidList.findA (String.string_dec x) l.
 
   Fixpoint compile_expr expr : option Clight.expr :=
@@ -74,7 +91,16 @@ Section Compile.
       end
     end
   .
-  (** vsub, vmul may not match with compcert's cop semantics *)
+  (** vsub, vmul may not agree with compcert's cop semantics *)
+
+  (* for function pointer call *)
+  Definition compile_expr_ptr tyargs expr : option Clight.expr :=
+    match expr with
+    | Var x =>
+      Some (Etempvar (s2p x) (Tptr0 (Tfunction tyargs Tlong0 cc_default)))
+    | _ => None
+    end
+  .
 
   Fixpoint compile_exprs (exprs: list Imp.expr) acc : option (list Clight.expr) :=
     match exprs with
@@ -84,43 +110,159 @@ Section Compile.
     end
   .
 
-  Fixpoint compile_stmt stmt : option Clight.statement :=
+  (* only check number of arguments, exploit Tlong <-> Tptr64 *)
+  Fixpoint cnt_args (tyargs: typelist) (args: list expr) : bool :=
+    match tyargs, args with
+    | Tnil, [] => true
+    | Tcons ty tys, e::es => cnt_args tys es
+    | _, _ => false
+    end
+  .
+
+  Fixpoint args_to_typelist (args: list expr) : typelist :=
+    match args with
+    | [] => Tnil
+    | h::t => Tcons Tlong0 (args_to_typelist t)
+    end
+  .
+
+  Fixpoint typelist_to_typs (tl: typelist) : list typ :=
+    match tl with
+    | Tnil => []
+    | Tcons h t => AST.Tlong :: (typelist_to_typs t)
+    end
+  .
+
+  (* Imp has no type, value is either int64/ptr64 -> sem_cast can convert *)
+  Fixpoint compile_stmt (g0: tgt_gdefs) stmt : option (tgt_gdefs * statement) :=
     match stmt with
     | Assign x e =>
-      do ex <- (compile_expr e); Some (Sset (s2p x) ex)
+      do ex <- (compile_expr e); Some (g0, Sset (s2p x) ex)
     | Seq s1 s2 =>
-      do cs1 <- (compile_stmt s1);
-      do cs2 <- (compile_stmt s2);
-      Some (Ssequence cs1 cs2)
+      do '(g1, cs1) <- (compile_stmt g0 s1);
+      do '(g2, cs2) <- (compile_stmt g1 s2);
+      Some (g2, Ssequence cs1 cs2)
     | If cond sif selse =>
       do cc <- (compile_expr cond);
-      do cif <- (compile_stmt sif);
-      do celse <- (compile_stmt selse);
-      Some (Sifthenelse cc cif celse)
+      do '(g1, cif) <- (compile_stmt g0 sif);
+      do '(g2, celse) <- (compile_stmt g1 selse);
+      Some (g2, Sifthenelse cc cif celse)
     | While cond body =>
       do cc <- (compile_expr cond);
-      do cbody <- (compile_stmt body);
-      Some (Swhile cc cbody)
+      do '(g1, cbody) <- (compile_stmt g0 body);
+      Some (g1, Swhile cc cbody)
     | Skip =>
-      Some Sskip
+      Some (g0, Sskip)
 
     | CallFun1 x f args =>
+      do al <- (compile_exprs args []);
+      Some
+        (g0,
+         Scall
+           (Some (s2p x))
+           (Evar (s2p f) (Tfunction (args_to_typelist al) Tlong0 cc_default))
+           al)
     | CallFun2 f args =>
+      do al <- (compile_exprs args []);
+      Some
+        (g0,
+         Scall
+           None
+           (Evar (s2p f) (Tfunction (args_to_typelist al) Tlong0 cc_default))
+           al)
+      
     | CallPtr1 x pe args =>
+      do al <- (compile_exprs args []);
+      do a <- compile_expr_ptr (args_to_typelist al) pe;
+      Some (g0, Scall (Some (s2p x)) a al)
     | CallPtr2 pe args =>
+      do al <- (compile_exprs args []);
+      do a <- compile_expr_ptr (args_to_typelist al) pe;
+      Some (g0, Scall None a al)
+
     | CallSys1 x f args =>
+      match ident_key (s2p f) g0 with
+      | Some gd =>
+        match gd with
+        | Gfun fd =>
+          match fd with
+          | External ef tyargs tyres cconv =>
+            do al <- (compile_exprs args []);
+            if (cnt_args tyargs al)
+            then
+              Some
+                (g0,
+                 Scall
+                   (Some (s2p x))
+                   (Evar (s2p f) (Tfunction tyargs tyres cconv))
+                   al)
+            else None
+          | _ => None
+          end
+        | _ => None
+        end
+      | None =>
+        do al <- (compile_exprs args []);
+        let tyargs := args_to_typelist al in
+        let sg := mksignature (typelist_to_typs tyargs) (Tret AST.Tlong) cc_default in
+        let fd := Gfun (External (EF_external f sg) tyargs Tlong0 cc_default) in
+        let g1 := ((s2p f), fd)::g0 in
+        Some
+          (g1,
+           Scall
+             (Some (s2p x))
+             (Evar (s2p f) (Tfunction tyargs Tlong0 cc_default))
+             al)
+      end
     | CallSys2 f args =>
+      match ident_key (s2p f) g0 with
+      | Some gd =>
+        match gd with
+        | Gfun fd =>
+          match fd with
+          | External ef tyargs tyres cconv =>
+            do al <- (compile_exprs args []);
+            if (cnt_args tyargs al)
+            then
+              Some
+                (g0,
+                 Scall
+                   None
+                   (Evar (s2p f) (Tfunction tyargs tyres cconv))
+                   al)
+            else None
+          | _ => None
+          end
+        | _ => None
+        end
+      | None =>
+        do al <- (compile_exprs args []);
+        let tyargs := args_to_typelist al in
+        let sg := mksignature (typelist_to_typs tyargs) (Tret AST.Tlong) cc_default in
+        let fd := Gfun (External (EF_external f sg) tyargs Tlong0 cc_default) in
+        let g1 := ((s2p f), fd)::g0 in
+        Some
+          (g1,
+           Scall
+             None
+             (Evar (s2p f) (Tfunction tyargs Tlong0 cc_default))
+             al)
+      end
 
     | Return1 r =>
-      do cr <- (compile_expr r); Some (Sreturn (Some cr))
+      do cr <- (compile_expr r); Some (g0, Sreturn (Some cr))
     | Return2 =>
-      Some (Sreturn None)
+      Some (g0, Sreturn None)
+
     | AddrOf x GN =>
-      Some (Sset (s2p x) (Eaddrof (Evar (s2p GN) Tlong0) Tlong0))
+      (* GN: global name, tgt_g may not contain -> resolved by linking *)
+      Some (g0, Sset (s2p x) (Eaddrof (Evar (s2p GN) Tlong0) Tlong0))
     | Load x pe =>
-      do cpe <- (compile_expr pe); Some (Sset (s2p x) (Ederef cpe Tlong0))
-    | Store X ve =>
-      do vpe <- (compile_expr ve); Some (Sassign (Evar (s2p X) Tlong0) vpe)
+      do cpe <- (compile_expr pe); Some (g0, Sset (s2p x) (Ederef cpe Tlong0))
+    | Store pe ve =>
+      do cpe <- (compile_expr pe);
+      do cve <- (compile_expr ve);
+      Some (g0, Sassign (Ederef cpe Tlong0) cve)
     end
   .
 
